Compiler/CompilationModel/ValidationHelpers.lean
@@ -79,8 +79,12 @@ def collectExprNames : Expr → List String
   | Expr.internalCall name args => name :: collectExprListNames args
   | Expr.arrayLength name => [name]
   | Expr.paramDynamicHeadWord name _ => [name]
+  | Expr.paramDynamicMemberLength name _
+  | Expr.paramDynamicMemberDataOffset name _ => [name]
+  | Expr.paramDynamicMemberElement name _ innerIndex => name :: collectExprNames innerIndex
   | Expr.arrayElement name index | Expr.arrayElementWord name index _ _
   | Expr.arrayElementDynamicWord name index _
+  | Expr.arrayElementDynamicDataOffset name index
   | Expr.arrayElementDynamicMemberDataOffset name index _
   | Expr.arrayElementDynamicMemberLength name index _ =>
       name :: collectExprNames index
